Syntax.v
@@ -1,0 +1,127 @@
+Require Import Coq.Strings.Ascii.
+Require Import Coq.Strings.String.
+Require Import Coq.Lists.List.
+Import ListNotations.
+Require Export WSpace.Bin.
+
+Inductive char : Type :=
+  | Space
+  | Tab
+  | LF.
+
+Inductive token : Type :=
+  | TPush (n : bin)
+  | TDup
+  | TCopy (n : bin)
+  | TSwap
+  | TDrop
+  | TSlide (n : bin)
+  | TAdd
+  | TSub
+  | TMul
+  | TDiv
+  | TMod
+  | TStore
+  | TRetrieve
+  | TLabel (l : bin)
+  | TCall (l : bin)
+  | TJmp (l : bin)
+  | TJz (l : bin)
+  | TJn (l : bin)
+  | TRet
+  | TEnd
+  | TPrintc
+  | TPrinti
+  | TReadc
+  | TReadi
+  | TError.
+
+Definition map_standard (a : ascii) : option char :=
+  match a with
+  | Ascii false false false false false true false false => Some Space (* ' ' *)
+  | Ascii true false false true false false false false => Some Tab (* '\t' *)
+  | Ascii false true false true false false false false => Some LF (* '\n' *)
+  | _ => None
+  end.
+Definition map_STL (a : ascii) : option char :=
+  match a with
+  | Ascii true true false false true false true false => Some Space (* 'S' *)
+  | Ascii false false true false true false true false => Some Tab (* 'T' *)
+  | Ascii false false true true false false true false => Some LF (* 'L' *)
+  | _ => None
+  end.
+
+Fixpoint scan (s : string) (map : ascii -> option char)
+    : list char :=
+  match s with
+  | EmptyString => []
+  | String a s' => match map a with
+                   | Some c => c :: scan s' map
+                   | None => scan s' map
+                   end
+  end.
+
+Fixpoint parse (cs : list char) : list token :=
+  let fix parse_arg' (cs : list char) (ctor : bin -> token) (b : bin)
+      : list token :=
+    match cs with
+    | Space :: cs' => parse_arg' cs' ctor (B0 :: b)
+    | Tab :: cs' => parse_arg' cs' ctor (B1 :: b)
+    | LF :: cs' => ctor b :: parse cs'
+    | [] => [TError]
+    end in
+  let parse_arg := fun cs ctor => parse_arg' cs ctor [] in
+  match cs with
+  | Space :: Space :: cs' => parse_arg cs' TPush
+  | Space :: LF :: Space :: cs' => TDup :: parse cs'
+  | Space :: Tab :: Space :: cs' => parse_arg cs' TCopy
+  | Space :: LF :: Tab :: cs' => TSwap :: parse cs'
+  | Space :: LF :: LF :: cs' => TDrop :: parse cs'
+  | Space :: Tab :: LF :: cs' => parse_arg cs' TSlide
+  | Tab :: Space :: Space :: Space :: cs' => TAdd :: parse cs'
+  | Tab :: Space :: Space :: Tab :: cs' => TSub :: parse cs'
+  | Tab :: Space :: Space :: LF :: cs' => TMul :: parse cs'
+  | Tab :: Space :: Tab :: Space :: cs' => TDiv :: parse cs'
+  | Tab :: Space :: Tab :: Tab :: cs' => TMod :: parse cs'
+  | Tab :: Tab :: Space :: cs' => TStore :: parse cs'
+  | Tab :: Tab :: Tab :: cs' => TRetrieve :: parse cs'
+  | LF :: Space :: Space :: cs' => parse_arg cs' TLabel
+  | LF :: Space :: Tab :: cs' => parse_arg cs' TCall
+  | LF :: Space :: LF :: cs' => parse_arg cs' TJmp
+  | LF :: Tab :: Space :: cs' => parse_arg cs' TJz
+  | LF :: Tab :: Tab :: cs' => parse_arg cs' TJn
+  | LF :: Tab :: LF :: cs' => TRet :: parse cs'
+  | LF :: LF :: LF :: cs' => TEnd :: parse cs'
+  | Tab :: LF :: Space :: Space :: cs' => TPrintc :: parse cs'
+  | Tab :: LF :: Space :: Tab :: cs' => TPrinti :: parse cs'
+  | Tab :: LF :: Tab :: Space :: cs' => TReadc :: parse cs'
+  | Tab :: LF :: Tab :: Tab :: cs' => TReadi :: parse cs'
+  | [] => []
+  | _ => [TError]
+  end.
+
+Example count :
+  let src := "CountSfromS1StoT10LLSSSTSSSSTTLSLSTLSTSSSTSTSLTLSSSSSTLTSSSSLSSSSTSTTLTSSTLTSSTSSSTSTLLSLSTSSSSTTLLSSSTSSSTSTLSLLLLL"%string in
+  let chars := [Space; Space; Space; Tab; LF; LF; Space; Space; Space; Tab;
+    Space; Space; Space; Space; Tab; Tab; LF; Space; LF; Space; Tab; LF; Space;
+    Tab; Space; Space; Space; Tab; Space; Tab; Space; LF; Tab; LF; Space; Space;
+    Space; Space; Space; Tab; LF; Tab; Space; Space; Space; Space; LF; Space;
+    Space; Space; Space; Tab; Space; Tab; Tab; LF; Tab; Space; Space; Tab; LF;
+    Tab; Space; Space; Tab; Space; Space; Space; Tab; Space; Tab; LF; LF; Space;
+    LF; Space; Tab; Space; Space; Space; Space; Tab; Tab; LF; LF; Space; Space;
+    Space; Tab; Space; Space; Space; Tab; Space; Tab; LF; Space; LF; LF; LF;
+    LF; LF] in
+  let tokens := [
+    TPush (Bin.of_nat_signed 1);
+    TLabel (Bin.of_string "C");
+    TDup; TPrinti;
+    TPush (Bin.of_nat_signed 10); TPrintc;
+    TPush (Bin.of_nat_signed 1); TAdd;
+    TDup; TPush (Bin.of_nat_signed 11); TSub; TJz (Bin.of_string "E");
+    TJmp (Bin.of_string "C");
+    TLabel (Bin.of_string "E");
+    TDrop;
+    TEnd] in
+  scan src map_STL = chars /\
+  parse chars = tokens.
+Proof. split; reflexivity. Qed.
